Cslib/Data/ComputableFresh.lean
@@ -1,0 +1,36 @@
+/-
+Copyright (c) 2025 Fabrizio Montesi. All rights reserved.
+Released under Apache 2.0 license as described in the file LICENSE.
+Authors: Fabrizio Montesi
+-/
+
+import Mathlib.Data.Finset.Basic
+import Mathlib.Data.Finset.Max
+import Mathlib.Data.Nat.Find
+import Mathlib.Data.Fintype.EquivFin
+import Mathlib.Order.SuccPred.Basic
+
+universe u
+
+/-- A type `α` has a computable `fresh` function if it is always possible, for any finite set of `α`, to compute a fresh element not in the set. -/
+class ComputableFresh (α : Type u) where
+  fresh : Finset α → α
+  fresh_notMem (s : Finset α) : fresh s ∉ s
+
+/-- `ℕ` has a computable fresh function. -/
+instance instComputableFreshNat : ComputableFresh ℕ where
+  -- We could also use Nat.find here.
+  fresh s :=
+    match s.max with
+    | ⊥ => 0
+    | some n => n.succ
+  fresh_notMem s := by
+    cases h : s.max
+    case bot =>
+      simp [Finset.max] at h
+      simp
+      exact h 0
+    case coe n =>
+      simp
+      have h' : s.max < ↑(n + 1) := by simp_all only [WithBot.coe_lt_coe, Nat.lt_add_one]
+      apply Finset.notMem_of_max_lt_coe h'
