Cslib/Syntax/HasAlphaEquiv.lean
@@ -1,0 +1,14 @@
+/-
+Copyright (c) 2025 Fabrizio Montesi. All rights reserved.
+Released under Apache 2.0 license as described in the file LICENSE.
+Authors: Fabrizio Montesi
+-/
+
+import Mathlib.Data.Rel
+
+/-- Typeclass for the α-equivalence notation `x =α y`. -/
+class HasAlphaEquiv (β : Type u) where
+  /-- α-equivalence relation for type β. -/
+  AlphaEquiv : Rel β β
+
+notation m:max " =α " n:max => HasAlphaEquiv.AlphaEquiv m n
