Cslib/Syntax/Substitution.lean
@@ -4,8 +4,9 @@ Released under Apache 2.0 license as described in the file LICENSE.
 Authors: Fabrizio Montesi
 -/
 
-/-- Class for substitution relations. WIP. -/
-class Substitution where
-  subst : α → β → α → α
+/-- Class for substitution relations. -/
+class Substitution (α : Type u) (β : Type v) where
+  /-- Substitution function. Replaces `x` in `t` with `t'`. -/
+  subst (t : α) (x : β) (t' : α) : α
 
 notation t:max "[" x ":=" t' "]" => Substitution.subst t x t'
